# baseURI: http://promsns.org/def/agr
# imports: http://creativecommons.org/schema.rdf
# imports: http://dublincore.org/2012/06/14/dcterms.rdf
# imports: http://purl.org/dc/elements/1.1/
# imports: http://www.w3.org/2004/02/skos/core
# imports: http://www.w3.org/ns/org.ttl
# imports: http://www.w3.org/ns/prov-o#
# imports: http://xmlns.com/foaf/0.1/

@prefix : <http://promsns.org/def/agr#> .
@prefix dc: <http://purl.org/dc/elements/1.1/> .
@prefix dcterms: <http://purl.org/dc/terms/> .
@prefix foaf: <http://xmlns.com/foaf/0.1/> .
@prefix org: <http://www.w3.org/ns/org#> .
@prefix owl: <http://www.w3.org/2002/07/owl#> .
@prefix prov: <http://www.w3.org/ns/prov#> .
@prefix rdf: <http://www.w3.org/1999/02/22-rdf-syntax-ns#> .
@prefix rdfs: <http://www.w3.org/2000/01/rdf-schema#> .
@prefix xsd: <http://www.w3.org/2001/XMLSchema#> .

<http://promsns.org/def/agr>
  rdf:type owl:Ontology ;
  dc:creator "Nicholas Car"^^xsd:string ;
  dcterms:created "2016-09-12"^^xsd:date ;
  dcterms:creator <http://promsns.org/id/person/nicholascar> ;
  dcterms:modified "2016-09-22"^^xsd:date ;
  rdfs:comment "This Agreements Ontology is designed to model 'agreements' which are social contracts that include licenses, laws, contracts, Memoranda of Understanding, standards and definitional metadata. Its purpose is to support data sharing by making explicit the relationships between agreements and data and agreements and Agents (people and organisations). Eventually it will also help with the interplay between different classes of agreements."^^xsd:string ;
  rdfs:label "Agreements ontology"^^xsd:string ;
  owl:imports <http://creativecommons.org/schema.rdf> ;
  owl:imports <http://dublincore.org/2012/06/14/dcterms.rdf> ;
  owl:imports dc: ;
  owl:imports <http://www.w3.org/2004/02/skos/core> ;
  owl:imports <http://www.w3.org/ns/org.ttl> ;
  owl:imports <http://www.w3.org/ns/prov-o#> ;
  owl:imports foaf: ;
  owl:versionInfo "v1.1"^^xsd:string ;
.
:Agreement
  rdf:type owl:Class ;
  rdfs:comment "A description of a set of required actions by particular agents"@en ;
  rdfs:label "Agreement"@en ;
  rdfs:subClassOf prov:Plan ;
  rdfs:subClassOf [
      rdf:type owl:Restriction ;
      owl:minCardinality "1"^^xsd:nonNegativeInteger ;
      owl:onProperty :requires ;
    ] ;
.
:MAY
  rdf:type :RequirementLevel ;
  rdfs:label "MAY"^^xsd:string ;
.
:MUST
  rdf:type :RequirementLevel ;
  rdfs:label "MUST"^^xsd:string ;
.
:MUST_NOT
  rdf:type :RequirementLevel ;
  rdfs:label "MUST NOT"^^xsd:string ;
.
:OPTIONAL
  rdf:type :RequirementLevel ;
  rdfs:label "OPTIONAL"^^xsd:string ;
.
:RECOMMENDED
  rdf:type :RequirementLevel ;
  rdfs:label "RECOMMENDED"^^xsd:string ;
.
:REQUIRED
  rdf:type :RequirementLevel ;
  rdfs:label "REQUIRED"^^xsd:string ;
.
:Requirement
  rdf:type owl:Class ;
  rdfs:comment "This class is analagous to the Creative Commons ontology formerly available. According to CC, a Requirement is \"an action that may or may not be requested of you\". In this ontology, it is only \"an action that may be requested of you\""@en ;
  rdfs:label "Requirement"@en ;
  rdfs:subClassOf <http://www.w3.org/2004/02/skos/core#Concept> ;
  rdfs:subClassOf prov:Plan ;
  rdfs:subClassOf [
      rdf:type owl:Restriction ;
      owl:cardinality "1"^^xsd:nonNegativeInteger ;
      owl:onProperty :requirementLevel ;
    ] ;
.
:RequirementLevel
  rdf:type owl:Class ;
  rdfs:comment "An RequirementLevel is the level at which an Agreement complels the Agents it affects to action. The initial instances of Imperative are taken from RFC2119."@en ;
  rdfs:label "Requirement Level"@en ;
  rdfs:subClassOf <http://www.w3.org/2004/02/skos/core#Concept> ;
.
:RequirementResolution
  rdf:type owl:Class ;
  rdfs:comment "An action that resolves requirements"@en ;
  rdfs:label "Requirement Resolution"@en ;
  rdfs:subClassOf <http://www.w3.org/2004/02/skos/core#Concept> ;
  rdfs:subClassOf prov:Activity ;
  rdfs:subClassOf [
      rdf:type owl:Restriction ;
      owl:cardinality "1"^^xsd:nonNegativeInteger ;
      owl:onProperty :satisfies ;
    ] ;
.
:SHALL
  rdf:type :RequirementLevel ;
  rdfs:label "SHALL"^^xsd:string ;
.
:SHALL_NOT
  rdf:type :RequirementLevel ;
  rdfs:label "SHALL NOT"^^xsd:string ;
.
:SHOULD
  rdf:type :RequirementLevel ;
  rdfs:label "SHOULD"^^xsd:string ;
.
:SHOULD_NOT
  rdf:type :RequirementLevel ;
  rdfs:label "SHOULD NOT"^^xsd:string ;
.
:hasScopeOf
  rdf:type owl:ObjectProperty ;
  rdfs:comment "This property indicates which Agent is affected by an Agreement. It is likely that the Agent will be a group (foaf:Group) or an Organization (org:Organisation) rather than an individual person and certainly not a machine Agent."@en ;
  rdfs:domain :Agreement ;
  rdfs:label "has scope of"@en ;
  rdfs:range prov:Agent ;
.
:requirementLevel
  rdf:type owl:ObjectProperty ;
  rdfs:comment "a Requirement has a requirementLevel of a RequirementLevel"@en ;
  rdfs:domain :Requirement ;
  rdfs:label "requirement level"@en ;
  rdfs:range :RequirementLevel ;
.
:requirementOf
  rdf:type owl:InverseFunctionalProperty ;
  rdfs:domain :Requirement ;
  rdfs:label "requirement of"^^xsd:string ;
  rdfs:range :Agreement ;
  rdfs:subPropertyOf dcterms:isPartOf ;
  owl:inverseOf :requires ;
.
:requires
  rdf:type owl:ObjectProperty ;
  rdfs:comment "an Agreement requires a Requirement"^^xsd:string ;
  rdfs:domain :Agreement ;
  rdfs:label "requires"^^xsd:string ;
  rdfs:range :Requirement ;
  rdfs:subPropertyOf dcterms:hasPart ;
  owl:inverseOf :requirementOf ;
.
:satisfiedBy
  rdf:type owl:InverseFunctionalProperty ;
  rdfs:comment "inverse of satisfies"@en ;
  rdfs:domain :Requirement ;
  rdfs:label "satisfied by"@en ;
  rdfs:range :RequirementResolution ;
  rdfs:subPropertyOf prov:influenced ;
  owl:inverseOf :satisfies ;
.
:satisfies
  rdf:type owl:ObjectProperty ;
  rdfs:comment "a Requirement Resolution satisfies a Requirement"@en ;
  rdfs:domain :RequirementResolution ;
  rdfs:label "satisfies"@en ;
  rdfs:range :Requirement ;
  rdfs:subPropertyOf prov:wasInfluencedBy ;
  owl:inverseOf :satisfiedBy ;
.
